Added less-than-or-equal PreOrder relation for trace and traces, and ensured that semantic commands return equal-or-greater set of traces.

Java/src/Semantics/SemCmd.v
@@ -19,11 +19,17 @@ Section Commands.
       (HSafe  : forall m, m <= n -> safe c P m s h t)
       (HSem   : c P n s big t (Some (s', (big', t')))),
       exists h', sa_mul h' frame big' /\ c P n s h t (Some (s', (h', t'))).
+  Definition increasing_traces (c : semCmdType) :=
+    forall P s s' h h' n t t'
+      (HSafe  : forall m, m <= n -> safe c P m s h t)
+      (HSem : c P n s h t (Some (s', (h', t')))),
+      traces_lte t t'.
 
   Record semCmd := {
     cmd_rel   :> Prog_wf -> nat -> stack -> heap -> traces -> option (stack * (heap * traces)) -> Prop;
     cmd_zero  :  forall P s h t cfg, ~(cmd_rel P 0 s h t cfg);
-    cmd_frame :  frame_property cmd_rel
+    cmd_frame :  frame_property cmd_rel;
+    cmd_trace :  increasing_traces cmd_rel
   }.
 
   Definition not_modifies (c : semCmdType) x : Prop :=
@@ -34,6 +40,19 @@ Section Commands.
   Proof.
     intros; apply cmd_zero.
   Qed.
+  
+  
+  Lemma semCmd_traces_lte : forall (c : semCmd) P s s' h h' t t' n
+    (HSafe  : forall m, m <= n -> safe c P m s h t) 
+    (HSem: c P n s h t (Some (s', (h', t')))),
+    traces_lte t t'. 
+  Proof.
+    intros.
+    intros k v Hmt.
+    edestruct (@cmd_trace c); try eassumption. 
+    exists x.
+    apply H.
+  Qed.
 
   Global Opaque sa_mul.
 
@@ -42,19 +61,24 @@ Section Commands.
   Program Definition later_cmd (c : semCmd) : semCmd := Build_semCmd
     (fun P n => match n return stack -> heap -> traces -> option (stack * (heap * traces)) -> Prop with
                   | O => fun _ _ _ _ => False
-                  | S n => c P n end) _ _.
+                  | S n => c P n end) _ _ _.
   Next Obligation.
     unfold frame_property; intros.
     destruct n as [| n]; unfold safe in HSafe; simpl in *; [contradiction |].
     eapply cmd_frame; eauto. 
     intros m HLe HFail; apply (HSafe (S m)); auto with arith.
   Qed.
-
+  Next Obligation.
+    unfold increasing_traces; intros.
+    destruct n as [| n]; unfold safe in HSafe; simpl in *; [contradiction |].
+    eapply cmd_trace; eauto.
+    intros m HLe HFail; apply (HSafe (S m)); auto with arith.
+  Qed.
   (* Skip *)
 
   Inductive skip_sem : semCmdType :=
   | s_ok : forall P s h t, skip_sem P 1 s h t (Some (s, (h, t))).
-  Program Definition skip_cmd := @Build_semCmd skip_sem _ _.
+  Program Definition skip_cmd := @Build_semCmd skip_sem _ _ _.
   Next Obligation.
     intros H. inversion H.
   Qed.
@@ -62,6 +86,11 @@ Section Commands.
     unfold frame_property; intros.
     inversion HSem; subst; clear HSem.
     exists h; auto using skip_sem.
+  Qed.
+  Next Obligation.
+    unfold increasing_traces; intros.
+    inversion HSem; subst; clear HSem.
+    reflexivity.
   Qed.
 
   (* Seq *)
@@ -77,7 +106,7 @@ Section Commands.
       c1 P n  s  h  t  (Some (s0, (h0, t0))) ->
       c2 P n0 s0 h0 t0 (Some (s1, (h1, t1))) ->
       seq_sem c1 c2 P (S (n + n0)) s h t (Some (s1, (h1, t1))).
-  Program Definition seq_cmd c1 c2 := @Build_semCmd (seq_sem c1 c2) _ _.
+  Program Definition seq_cmd c1 c2 := @Build_semCmd (seq_sem c1 c2) _ _ _.
   Next Obligation.
     intros H; inversion H.
   Qed.
@@ -89,6 +118,19 @@ Section Commands.
     + edestruct (@cmd_frame c2) with(n:=n1) as [hr [HFrame1 HSem1]]...
       intros m HLe HFail; apply HSafe with (S (n0 + m)); [omega | ]...
   Qed.
+  Next Obligation with eauto using seq_sem.
+    unfold increasing_traces; intros.
+    inversion HSem; subst; clear HSem.
+    assert (traces_lte t t1). {
+      apply semCmd_traces_lte in H6; [ apply H6 |].
+      intros m HLe HFail; apply HSafe with (S m); [omega | ]...
+    }
+    assert (traces_lte t1 t'). {
+      apply semCmd_traces_lte in H8; [ apply H8 |].
+      intros m HLe HFail; apply HSafe with (S (n0 + m)); [omega | ]...
+	}
+    transitivity t1; assumption.
+  Qed.    
 
   (* Nondet *)
   Inductive nondet_sem (c1 c2 : semCmd) : semCmdType :=
@@ -104,7 +146,7 @@ Section Commands.
   | nondet_okR   : forall P n s s' h h' t t',
       c2 P n s h t (Some (s', (h', t'))) ->
       nondet_sem c1 c2 P (S n) s h t (Some (s', (h', t'))).
-  Program Definition nondet_cmd c1 c2 := @Build_semCmd (nondet_sem c1 c2) _ _.
+  Program Definition nondet_cmd c1 c2 := @Build_semCmd (nondet_sem c1 c2) _ _ _.
   Next Obligation.
     intros H; inversion H.
   Qed.
@@ -116,6 +158,14 @@ Section Commands.
     + edestruct (@cmd_frame c2) as [h0 [HFrame0 HSem0]]...
       intros m HLe HFail; apply HSafe with (S m); [omega |]...
   Qed.
+  Next Obligation with eauto using nondet_sem.
+    unfold increasing_traces; intros.
+    inversion HSem; subst; clear HSem.
+    + apply semCmd_traces_lte in H5; [ apply H5 |].
+      intros m HLe HFail; apply HSafe with (S m); [omega |]...
+    + apply semCmd_traces_lte in H5; [ apply H5 |].
+      intros m HLe HFail; apply HSafe with (S m); [omega |]...
+  Qed.    
 
   (* Kleene star *)
   Inductive kleene_sem (c : semCmd) : semCmdType :=
@@ -132,7 +182,7 @@ Section Commands.
       c P n s h t (Some (s0, (h0, t0))) ->
       kleene_sem c P n0 s0 h0 t0 (Some (s1, (h1, t1))) ->
       kleene_sem c P (S (n + n0)) s h t (Some (s1, (h1, t1))).
-  Program Definition kleene_cmd c := @Build_semCmd (kleene_sem c) _ _.
+  Program Definition kleene_cmd c := @Build_semCmd (kleene_sem c) _ _ _.
   Next Obligation.
     intros H; inversion H.
   Qed.
@@ -145,6 +195,19 @@ Section Commands.
     + destruct (IHHSem (eq_refl _) h' HFrame0) as [hr [HFrame1 HSem1]]...
       intros m HLe HFail; apply HSafe with (S (n + m)); [omega |]...
   Qed.
+  Next Obligation with eauto using kleene_sem.
+    unfold increasing_traces; intros.
+    remember (Some (s', (h', t'))) as cfg; induction HSem;
+    inversion Heqcfg; subst; intros; clear Heqcfg...
+    reflexivity.
+    assert (traces_lte t t0). {
+      apply semCmd_traces_lte in H; [ apply H |].
+      intros m HLe HFail; apply HSafe with (S m); [omega |]...
+    }
+    transitivity t0; [apply H0 |].
+    apply IHHSem; [| reflexivity].
+    intros m HLe HFail; apply HSafe with (S (n + m)); [omega |]...
+  Qed.
 
   (* TODO: update the description
      assume command -- this command is a bit of a hack that just skips if
@@ -152,7 +215,7 @@ Section Commands.
      using nondeterministic choice/Kleene star *)
   Inductive assume_sem (p : vlogic) : semCmdType :=
   | assume_ok : forall P s h t, p s -> assume_sem p P 1 s h t (Some (s, (h, t))).
-  Program Definition assume_cmd P := @Build_semCmd (assume_sem P) _ _.
+  Program Definition assume_cmd P := @Build_semCmd (assume_sem P) _ _ _.
   Next Obligation.
     intros H; inversion H.
   Qed.
@@ -160,6 +223,11 @@ Section Commands.
     unfold frame_property; simpl; intros.
     remember (Some (s', (big', t'))) as cfg; induction HSem.
     inversion Heqcfg; subst; eauto using assume_sem.
+  Qed.
+  Next Obligation.
+    unfold increasing_traces; intros.
+    inversion HSem; subst. 
+    reflexivity.
   Qed.
 
   Lemma assume_inv P e n s s0 h h0 t t0 (HSem : assume_cmd e P n s h t (Some (s0, (h0, t0)))) : 
@@ -174,13 +242,18 @@ Section Commands.
     assert_sem p P 1 s h t (Some (s, (h, t)))
   | assert_fail : forall P s h t (HNP : ~p s),
     assert_sem p P 1 s h t None.
-  Program Definition assert_cmd p := @Build_semCmd (assert_sem p) _ _.
+  Program Definition assert_cmd p := @Build_semCmd (assert_sem p) _ _ _.
   Next Obligation.
     intros H; inversion H.
   Qed.
   Next Obligation.
     unfold frame_property; simpl; intros.
     inversion HSem; subst; eauto using assert_sem.
+  Qed.
+  Next Obligation.
+    unfold increasing_traces; intros.
+    inversion HSem; subst.
+    reflexivity.
   Qed.
 
   (* |= {p}c{q} *)
